add contract intro thm and refinement thm

complete-theory/compositionalityScript.sml
@@ -8,6 +8,11 @@ val _ = add_rule
   block_style = (AroundEachPhrase, (PP.INCONSISTENT, 2))};
 
 val _ = add_rule
+  {term_name = "Interpretation_S", fixity = Closefix,
+  pp_elements = [TOK "⟨", TM, TOK "⟩MS"], paren_style = OnlyIfNecessary,
+  block_style = (AroundEachPhrase, (PP.INCONSISTENT, 2))};
+
+val _ = add_rule
   {term_name = "Assertional", fixity = Closefix,
   pp_elements = [TOK "Assertional(", TM, TOK ")"], paren_style = OnlyIfNecessary,
   block_style = (AroundEachPhrase, (PP.INCONSISTENT, 2))};
@@ -40,31 +45,36 @@ val _ = add_rule {block_style = (AroundEachPhrase, (PP.INCONSISTENT, 2)),
                   fixity = Infix(NONASSOC, 425),
                   paren_style = OnlyIfNecessary,
                   pp_elements = [TOK "ₓ"],
-                  term_name = "Comp"}
+                  term_name = "Composition"}
 
 Datatype:
-  Term = Implements C S | Assertional S | Refines S S
-  ;
-  C = Q α | Comp C C
-  ;
-  S = P (α set) | And S S | Contract S S | Parallell S S
+  C = Q α | Composition C C
+End
+
+Datatype:
+  S = P (α set) | And S S | Contract S S | Parallell S S | Assertional S
 End
 
 Definition C_M:
     C_M (Q α) = {α}
-  ∧ C_M (Comp c1 c2) = (C_M c1) ∩ (C_M c2)
+  ∧ C_M (c1 ₓ c2) = (C_M c1) ∩ (C_M c2)
 End
 
-
-
 (* TODO Contract, Parallell *)
-Definition S_M:
+Definition Interpretation:
     (S_M (P α) = {α})
   ∧ (S_M (And s1 s2) = (S_M s1) ∩ (S_M s2))
+  ∧ (S_M (Contract s1 s2) = {b | ∀b'. b' ∈ S_M s1 ⇒ b' ∩ b ∈ S_M s2})
+  ∧ (S_M (Parallell s1 s2) = {a ∩ b | a ∈ (S_M s1) ∧ b ∈ (S_M s2)})
+  ∧ (S_M (Assertional s) = S_M s)
 End
 
 Definition Impl:
-  Impl (c:α C) (s:α S) = if C_M c ∈ S_M s then T else F
+    (Impl (c:α C) (s:α S) = if C_M c ∈ S_M s then T else F)
+End
+
+Definition Refines:
+  Refines (s1:α S) (s2:α S) = if S_M s1 ⊆ S_M s2 then T else F
 End
 
 Theorem IMPL_AX_THM:
@@ -102,7 +112,42 @@ Proof
   rw[]
 QED
 
+Theorem CONTRACT_ELIM_THM:
+  ∀c1 c2 s1 s2. Impl c1 s1 ∧ Impl c2 (s1, s2) ⇒ Impl (Composition c1 c2) s2
+Proof
+  EVAL_TAC >>
+  rw[]
+QED
+
+Theorem SPEC_CONTRACT_INTRO_THM:
+  ∀c2 s1 s2. (∀q0. q0 ∈ S_M s1 ⇒ (q0 ∩ C_M c2) ∈ S_M s2) ⇒ Impl c2 (s1,s2)
+Proof
+  EVAL_TAC >>
+  rw[]
+QED
+
+Theorem REFINEMENT_THM:
+  ∀c s1 s2. Impl c s1 ∧ Refines s1 s2 ⇒ Impl c s2
+Proof
+  EVAL_TAC >>
+  metis_tac[pred_setTheory.SUBSET_DEF, pred_setTheory.SUBSET_TRANS]
+QED
+
 (*
+Theorem CONTRACT_INTRO_THM:
+  ∀c2 s1 s2. (∀c1. Impl c1 s1 ⇒ Impl (Composition c1 c2) s2) ⇒ Impl c2 (s1,s2)
+Proof
+  EVAL_TAC
+  rw[]
+
+QED
+*)
+
+(*
+Context menu
+
+Pallet
+        
 ax
 and-introduction
 and-elimination-1
